$\int \frac {dx}{e^x+e^{-x}} = \int \frac {e^x}{e^{2x}+1}dx = \int \frac {e^x}{u^2+1} . \frac {du}{e^x} = \int \frac {du}{u^2+1} = \tan ^{-1}(u)+c$
> solved by substitution using $u = e^x$,  $du=e^xdx$ and $dx = \frac {du}{e^x}$


$\int x^{3}*e^{x^4}$  |  $\int\frac{x^3e^udu}{4x^3} = \frac{1}{4}\int e^udu =\frac{e^u}{4}+c =\frac{e^{x^4}}{4}+c$  
$u=x^4$
$\frac{du}{4x^3}=dx$

a) $$\frac {\sqrt {4-x^2}}{x^2}dx = \int \frac {\sqrt {4-(2\sin t)^2}}{(2.\sin(t))^2} . 2\cos(t)dt = $$$$ \int \frac {\sqrt {4-4\sin^2(t).2\cos(t)dt}}{4\sin^2(t)} = \int \frac {\sqrt{4(1-\sin^2(t).\cos(t)}}{2\sin^2(t)}dt = $$ $$\int \frac {2.\cos(t).\cos(t)}{2\sin^2(t)} = \int \frac {\cos^2(t)}{\sin^2(t)} = \int \cot^2(t) = $$ $$\int \csc^2(t) -1dt = -\cot(t) -t +c = \frac {-\sqrt {4-x}}{x} - \sin^{-1} \frac {x}{2} + c$$
$x = 2.\sin(t)$ and $dx=2\cos(t)dt$

